inversion/c/montgomery_divstep/p384_32_test.c
@@ -1,0 +1,2 @@
+#include "p384_32.c"
+#include "test_template.c"
