inversion/c/solinas_divstep/p521_64.c
@@ -1,0 +1,9 @@
+#include "../../fiat-c/src/p521_64.c"
+
+#define LIMBS 9 /* amount of limbs pr. large integer in montgomery domain, see montgomery_inversion */
+#define WORD uint64_t
+#define WORDSIZE 64 /* wordsize */
+#define LEN_PRIME 521 /* length of the prime in bits */
+#define CURVE_DESCRIPTION fiat_p521
+
+#include "template.c"
