inversion/c/solinas_jumpdivstep/p448_solinas_64_test.c
@@ -1,0 +1,2 @@
+#include "p448_solinas_64.c"
+#include "test_template.c"
