inversion/c/solinas_test_template.c
@@ -1,0 +1,52 @@
+#include <stdio.h>
+#include <stdlib.h>
+#include <string.h>
+#include <inttypes.h>
+#include <time.h>
+
+#define MAKE_FN_NAME1(x,y) x ## y
+#define MAKE_FN_NAME(x,y) MAKE_FN_NAME1(x,y)
+
+#define SAT_FROM_BYTES MAKE_FN_NAME(CURVE_DESCRIPTION,_sat_from_bytes)
+#define FROM_BYTES MAKE_FN_NAME(CURVE_DESCRIPTION,_from_bytes)
+#define TO_BYTES MAKE_FN_NAME(CURVE_DESCRIPTION,_to_bytes)
+
+int main() {
+  WORD res[LIMBS], out[LIMBS], g[SAT_LIMBS], g1[LIMBS];
+  uint8_t a[BYTES];
+
+  int seed = time(0);
+  srand(seed);
+  printf("%i\n", seed);	
+	
+  for (int j = 0; j < 10000; j++) {
+    int i;
+    for (i = 0; i < BYTES; i++) {
+      a[i] = rand() % 256;
+      if (i > BYTES - 8) a[i] = 0;
+    }
+		
+    SAT_FROM_BYTES(g,a);
+    FROM_BYTES(g1,a);
+	
+    inverse(out,g);
+		
+    MUL(res,out,g1);
+    TO_BYTES(a,res);
+		
+    if (a[0] != 1) {
+			/* printf("%" PRIu8 " ", a[0]); */
+      printf("FAIL\n");
+      return 2;
+    }
+    for (i = 1; i < BYTES; i++) {
+      if (a[i] != 0) {
+				/* printf("%" PRIu8 " ", a[i]); */
+        printf("FAIL\n");
+        return 1;
+      }
+    }
+  }
+  printf("PASS\n");
+  return 0;
+}
