src/Arithmetic/BYInvJump.v
@@ -1,0 +1,607 @@
+Require Import Coq.Strings.String.
+Require Import Coq.Bool.Bool.
+Require Import Coq.ZArith.ZArith.
+Require Import Coq.Lists.List.
+Require Import Coq.nsatz.Nsatz.
+Require Import Coq.micromega.Lia.
+Require Import Crypto.Arithmetic.UniformWeight.
+Require Import Crypto.Arithmetic.Saturated.
+Require Import Crypto.Arithmetic.Core.
+Require Import Crypto.Arithmetic.WordByWordMontgomery.
+
+Require Import Crypto.Util.LetIn.
+Require Import Crypto.Util.ListUtil.
+Require Import Crypto.Util.ZUtil.Notations.
+Require Import Crypto.Arithmetic.Partition.
+Require Import Crypto.Util.Decidable.
+Require Import Crypto.Util.ZUtil.Definitions.
+Require Import Crypto.Util.ZUtil.TruncatingShiftl.
+Require Import Crypto.Util.ZUtil.Modulo.
+Require Import Crypto.Util.ZUtil.Testbit.
+Require Import Crypto.Util.ZUtil.Shift.
+Require Import Crypto.Util.ZUtil.Div.
+Require Import Crypto.Util.ZUtil.Lor.
+Require Import Crypto.Util.ZUtil.Land.
+Require Import Crypto.Util.ZUtil.ArithmeticShiftr.
+Require Import Crypto.Util.ZUtil.Pow.
+Require Import Crypto.Util.ZUtil.LandLorShiftBounds.
+Require Import Crypto.Util.ZUtil.SignBit.
+Require Import Crypto.Util.ZUtil.SignExtend.
+Require Import Crypto.Util.ZUtil.TwosComplement.
+Require Import Crypto.Util.ZUtil.TwosComplementMul.
+Require Import Crypto.Arithmetic.ModOps.
+
+Require Import Crypto.Util.ZUtil.Tactics.SolveRange.
+Require Import Crypto.Util.ZUtil.Tactics.PullPush.Modulo.
+Require Import Crypto.Util.ZUtil.Tactics.SolveTestbit.
+
+Require Import Crypto.Arithmetic.BYInv.
+
+Import Positional.
+Import ListNotations.
+Import Definitions.
+Import Crypto.Util.ZUtil.Notations.
+Import WordByWordMontgomery.
+
+Local Open Scope Z.
+
+Local Coercion Z.of_nat : nat >-> Z.
+
+Definition sat_ones m n :=
+  repeat (2 ^ m - 1) n.
+
+Definition sat_is_neg machine_wordsize n a :=
+  nth_default 0 a (n - 1) >> (machine_wordsize - 1).
+
+(*Saturated multiplication of multi-limb integers *)
+Local Definition sat_mul machine_wordsize n1 n2 f g :=
+  fst (Rows.mul (uweight machine_wordsize) (2^machine_wordsize) n1 n2 f g).
+
+Definition sat_arithmetic_shiftr machine_wordsize n f k :=
+  (map
+     (fun i =>
+        ((nth_default 0 f i) >> k) |' (Z.truncating_shiftl machine_wordsize
+                                                           (nth_default 0 f (i + 1))
+                                                           (machine_wordsize - k)))
+     (seq 0 (n - 1)))
+    ++ [Z.arithmetic_shiftr machine_wordsize (nth_default 0 f (n - 1)) k].
+
+(* Extends a multi-limb integer in twos complement to a new base *)
+Definition sat_sign_extend machine_wordsize old_base new_base a :=
+  let high_limb := nth_default 0 a (old_base - 1) in
+  let cond := Z.sign_bit machine_wordsize high_limb in
+  dlet parity := Z.zselect cond 0 (2^machine_wordsize - 1) in
+        let padding := repeat parity (new_base - old_base) in
+        a ++ padding.
+
+
+
+Module WordByWordMontgomery.
+  Import WordByWordMontgomery.WordByWordMontgomery.
+
+  (* Converts a wordsized integer to montgomery domain *)
+  Definition twosc_word_to_montgomery machine_wordsize n m m' a :=
+    dlet cond := Z.twos_complement_neg machine_wordsize a in
+    dlet a_opp := Z.twos_complement_opp machine_wordsize a in
+    dlet a_enc := encodemod machine_wordsize n m m' a in
+    dlet a_opp_enc := encodemod machine_wordsize n m m' (a_opp) in
+    dlet a_opp_enc_opp := oppmod machine_wordsize n m (a_opp_enc) in
+    dlet res := select cond a_enc a_opp_enc_opp in res.
+
+  (* Converts a wordsize integer to montgomery domain (without multiplying by R2) *)
+  Definition twos_complement_word_to_montgomery_no_encode machine_wordsize n m a :=
+    dlet cond := Z.twos_complement_neg machine_wordsize a in
+    dlet a_opp := Z.twos_complement_opp machine_wordsize a in
+    dlet a_enc := Partition.partition (uweight machine_wordsize) n a in
+    dlet a_opp_enc := Partition.partition (uweight machine_wordsize) n a_opp in
+    dlet a_opp_enc_opp := oppmod machine_wordsize n m (a_opp_enc) in
+    dlet res := select cond a_enc a_opp_enc_opp in res.
+
+  Definition twosc_word_mod_m machine_wordsize n m a :=
+    dlet cond := Z.twos_complement_neg machine_wordsize a in
+          dlet a' := Z.zselect cond a (Z.twos_complement_opp machine_wordsize a) in
+                       let a'' := extend_to_length 1 n [a'] in
+                       let a''_opp := oppmod machine_wordsize n m a'' in
+                       select cond a'' a''_opp.
+
+End WordByWordMontgomery.
+
+Definition sat_word_bits machine_wordsize a :=
+  nth_default 0 a 0 mod 2^(machine_wordsize - 2).
+
+Definition sat_mod_word machine_wordsize n a :=
+  let cond := sat_is_neg machine_wordsize n a in
+  let a' := select cond a (sat_opp machine_wordsize n a) in
+  let t := (nth_default 0 a' 0) in
+  let res := Z.zselect cond t (Z.twos_complement_opp machine_wordsize t) in res.
+
+
+Definition sat_twos_complement_mul machine_wordsize na nb nab a b :=
+  firstn nab (fst (Rows.mul (uweight machine_wordsize) (2^machine_wordsize) nab (2 * nab)
+                            (sat_sign_extend machine_wordsize na nab a) (sat_sign_extend machine_wordsize nb nab b))).
+
+Definition sat_twos_complement_mul_full machine_wordsize na nb a b :=
+  sat_twos_complement_mul machine_wordsize na nb (na + nb) a b.
+
+Definition word_sat_mul machine_wordsize n (a : Z) b :=
+  sat_twos_complement_mul_full machine_wordsize 1 n [a] b.
+
+Definition twos_complement_word_full_divstep_aux machine_wordsize (data : Z * Z * Z * Z * Z * Z * Z) :=
+  let '(d,f,g,u,v,q,r) := data in
+  let cond := Z.land (Z.twos_complement_pos machine_wordsize d) (g mod 2) in
+  dlet d' := Z.zselect cond d (Z.twos_complement_opp machine_wordsize d) in
+  dlet f' := Z.zselect cond f g in
+  dlet g' := Z.zselect cond g (Z.twos_complement_opp machine_wordsize f) in
+  dlet u' := Z.zselect cond u q in
+  dlet v' := Z.zselect cond v r in
+  let u'':= (u' + u') mod 2^machine_wordsize in
+  let v'':= (v' + v') mod 2^machine_wordsize in
+  dlet q' := Z.zselect cond q (Z.twos_complement_opp machine_wordsize u) in
+  dlet r' := Z.zselect cond r (Z.twos_complement_opp machine_wordsize v) in
+  let g0 := g' mod 2 in
+  let d'' := (1 + d') mod 2^machine_wordsize in
+  dlet f'' := Z.zselect g0 0 f' in
+  let g'' := Z.arithmetic_shiftr1 machine_wordsize ((g' + f'') mod 2^machine_wordsize) in
+  dlet u''' := Z.zselect g0 0 u' in
+  dlet v''' := Z.zselect g0 0 v' in
+  let q'' := (q' + u''') mod 2^machine_wordsize in
+  let r'' := (r' + v''') mod 2^machine_wordsize in
+  (d'',f',g'',u'',v'',q'',r'').
+
+Definition twos_complement_word_full_divstep machine_wordsize d f g u v q r :=
+  twos_complement_word_full_divstep_aux machine_wordsize (d, f, g, u, v, q, r).
+
+Definition divstep_spec_full' d f g u v q r :=
+  if (0 <? d) && Z.odd g
+  then (1 - d, g, (g - f) / 2,
+        2 * q, 2 * r, q - u, r - v)
+  else (1 + d, f, (g + (g mod 2) * f) / 2,
+        2 * u, 2 * v, q + (g mod 2) * u, r + (g mod 2) * v).
+
+Module UnsaturatedSolinas.
+  Section __.
+      Context (limbwidth_num limbwidth_den : Z)
+              (limbwidth_good : 0 < limbwidth_den <= limbwidth_num)
+              (machine_wordsize : Z)
+              (s : Z)
+              (c : list (Z*Z))
+              (n : nat)
+              (sat_limbs : nat)
+              (word_sat_mul_limbs : nat)
+              (idxs : list nat)
+              (balance : list Z).
+
+  Definition word_to_solina a :=
+    dlet cond := Z.twos_complement_neg machine_wordsize a in
+    dlet a_opp := Z.twos_complement_opp machine_wordsize a in
+    dlet a_enc := encodemod limbwidth_num limbwidth_den s c n a in
+    dlet a_opp_enc := encodemod limbwidth_num limbwidth_den s c n (a_opp) in
+    dlet a_opp_enc_opp := oppmod limbwidth_num limbwidth_den n balance (a_opp_enc) in
+    dlet a_opp_enc_opp_carry := carrymod limbwidth_num limbwidth_den s c n idxs a_opp_enc_opp in
+    dlet res := select cond a_enc a_opp_enc_opp_carry in res.
+
+  Definition outer_loop_body f g (v r : list Z) :=
+    let '(_,f1,g1,u1,v1,q1,r1) := fold_right (fun i data => twos_complement_word_full_divstep_aux machine_wordsize data) (1,nth_default 0 f 0,nth_default 0 g 0,1,0,0,1) (seq 0 (Z.to_nat (machine_wordsize - 2))) in
+    dlet f2 := word_sat_mul machine_wordsize sat_limbs u1 f in
+    dlet f3 := word_sat_mul machine_wordsize sat_limbs v1 g in
+    dlet g2 := word_sat_mul machine_wordsize sat_limbs q1 f in
+    dlet g3 := word_sat_mul machine_wordsize sat_limbs r1 g in
+    dlet f4 := BYInv.sat_add machine_wordsize word_sat_mul_limbs f2 f3 in
+    dlet g4 := BYInv.sat_add machine_wordsize word_sat_mul_limbs g2 g3 in
+    dlet f5 := sat_arithmetic_shiftr machine_wordsize word_sat_mul_limbs f4 (machine_wordsize - 2) in
+    dlet g5 := sat_arithmetic_shiftr machine_wordsize word_sat_mul_limbs g4 (machine_wordsize - 2) in
+    dlet f6 := firstn sat_limbs f5 in
+    dlet g6 := firstn sat_limbs g5 in
+    dlet u2 := word_to_solina u1 in
+    dlet v02 := word_to_solina v1 in
+    dlet q2 := word_to_solina q1 in
+    dlet r02 := word_to_solina r1 in
+    dlet v2 := carry_mulmod limbwidth_num limbwidth_den s c n idxs u2 v in
+    dlet v3 := carry_mulmod limbwidth_num limbwidth_den s c n idxs v02 r in
+    dlet r2 := carry_mulmod limbwidth_num limbwidth_den s c n idxs q2 v in
+    dlet r3 := carry_mulmod limbwidth_num limbwidth_den s c n idxs r02 r in
+    dlet v4 := addmod limbwidth_num limbwidth_den n v2 v3 in
+    dlet v5 := carrymod limbwidth_num limbwidth_den s c n idxs v4 in
+    dlet r4 := addmod limbwidth_num limbwidth_den n r2 r3 in
+    dlet r5 := carrymod limbwidth_num limbwidth_den s c n idxs r4 in
+    (f6, g6, v, r).
+  End __.
+End UnsaturatedSolinas.
+  
+
+(** Section about arithmetic right shift *)
+
+Lemma sat_arithmetic_shiftr_0 machine_wordsize n f
+      (Hm : 0 < machine_wordsize)
+      (Hn : (0 < n)%nat)
+      (Hf : length f = n)
+      (Hf2 : forall z, In z f -> 0 <= z < 2^machine_wordsize) :
+  sat_arithmetic_shiftr machine_wordsize n f 0 = f.
+Proof.
+  assert (0 < 2 ^ machine_wordsize) by (apply Z.pow_pos_nonneg; lia).
+  unfold sat_arithmetic_shiftr.
+  rewrite Z.arithmetic_shiftr_0 by
+      (try apply nth_default_preserves_properties; try assumption; lia).
+  rewrite <- (map_nth_default_seq 0 n f) at 2 by assumption; destruct n; [lia|].
+  rewrite seq_snoc, map_app.
+  apply f_equal2; replace (S n - 1)%nat with n by lia; try reflexivity.
+  apply map_seq_ext; try lia; intros i Hi.
+  rewrite Z.shiftr_0_r, Z.truncating_shiftl_large, Z.lor_0_r, Nat.add_0_r by lia.
+  reflexivity. Qed.
+
+Lemma sat_arithmetic_shiftr_1 machine_wordsize n f
+      (Hm : 0 < machine_wordsize)
+      (Hf2 : forall z, In z f -> 0 <= z < 2^machine_wordsize) :
+  sat_arithmetic_shiftr machine_wordsize n f 1 =
+  sat_arithmetic_shiftr1 machine_wordsize n f.
+Proof.
+  assert (0 < 2 ^ machine_wordsize) by (apply Z.pow_pos_nonneg; lia).
+  unfold sat_arithmetic_shiftr, sat_arithmetic_shiftr1.
+  rewrite Z.arithmetic_shiftr_1 by
+      (try apply nth_default_preserves_properties; try assumption; lia).
+  reflexivity. Qed.
+
+Lemma sat_arithmetic_shiftr_sat_arithmetic_shiftr1 machine_wordsize n (f : list Z) k
+      (Hn : (0 < n)%nat)
+      (Hf : length f = n)
+      (Hk : 0 <= k < machine_wordsize)
+      (Hf2 : forall z, In z f -> 0 <= z < 2^machine_wordsize) :
+  sat_arithmetic_shiftr machine_wordsize n
+                        (sat_arithmetic_shiftr1 machine_wordsize n f) k =
+  sat_arithmetic_shiftr machine_wordsize n f (k + 1).
+Proof.
+  assert (0 < 2 ^ machine_wordsize) by (apply Z.pow_pos_nonneg; lia).
+  unfold sat_arithmetic_shiftr, sat_arithmetic_shiftr1.
+  rewrite nth_default_app, map_length, seq_length.
+  destruct (lt_dec (n - 1) (n - 1)); try lia.
+  replace (n - 1 - (n - 1))%nat with 0%nat by lia.
+  rewrite nth_default_cons, Z.arithmetic_shiftr_arithmetic_shiftr1
+    by (try (apply nth_default_preserves_properties; [assumption|Z.solve_range]); lia).
+  apply f_equal2; try reflexivity. apply map_seq_ext; try lia; intros i Hi.
+  rewrite !nth_default_app, map_length, seq_length.
+  destruct (lt_dec i (n - 1)); 
+    destruct (lt_dec (i + 1) (n - 1)); try lia.
+  - rewrite !(map_nth_default _ _ _ _ 0%nat 0) by (rewrite seq_length; lia).
+    rewrite !nth_default_seq_inbounds by lia.
+    rewrite Nat.add_0_r, Z.shiftr_lor, Z.shiftr_shiftr by lia.
+    rewrite Z.add_comm, <- Z.lor_assoc. apply f_equal2; try reflexivity.
+    rewrite Z.truncating_shiftl_lor by lia.
+    rewrite Z.truncating_shiftl_truncating_shiftl by lia.
+    Z.solve_using_testbit; rewrite (Z.testbit_neg_r _ (n1 - _)), orb_false_r, ?orb_false_l by lia; 
+      apply f_equal2; try lia.
+    all: apply f_equal2; try reflexivity; lia. 
+  - assert (E : (i + 1 = n - 1)%nat) by lia.
+    rewrite !(map_nth_default _ _ _ _ 0%nat 0) by (rewrite seq_length; lia).
+    rewrite !nth_default_seq_inbounds by lia; simpl; rewrite Nat.add_0_r.
+    rewrite E. replace (n - 1 - (n - 1))%nat with 0%nat by lia.
+    rewrite nth_default_cons, Z.shiftr_lor, Z.shiftr_shiftr, Z.add_comm by lia.
+    rewrite <- Z.lor_assoc.
+    apply f_equal2; [reflexivity|].
+    Z.solve_using_testbit. 
+    apply nth_default_preserves_properties; [assumption|lia]. Qed.
+
+Local Fixpoint iter_sat_arithmetic_shiftr1 m n f k :=
+  match k with
+  | 0%nat => f
+  | 1%nat => sat_arithmetic_shiftr1 m n f
+  | S k => iter_sat_arithmetic_shiftr1 m n (sat_arithmetic_shiftr1 m n f) k
+  end.
+
+Lemma iter_sat_arithmetic_shiftr_S m n f k :
+  iter_sat_arithmetic_shiftr1 m n f (S k)
+  = iter_sat_arithmetic_shiftr1 m n (sat_arithmetic_shiftr1 m n f) k.
+Proof. destruct k; reflexivity. Qed.
+
+Lemma sat_arithmetic_shiftr_bound m n f
+      (Hm : 0 <= m)
+      (Hf : forall z, In z f -> 0 <= z < 2 ^ m) :
+  forall y, In y (sat_arithmetic_shiftr1 m n f) -> 0 <= y < 2 ^ m.
+Proof.
+  intros y H; unfold sat_arithmetic_shiftr1 in H.
+  assert (H1 : 0 <= 0 < 2 ^ m) by Z.solve_range.
+  apply in_app_iff in H. destruct H; simpl in H.
+  - apply in_map_iff in H; destruct H as [i [H H0] ]; rewrite <- H.
+    pose proof nth_default_preserves_properties _ f i 0 Hf H1;
+      simpl in H2; Z.solve_range.
+  - destruct H as [H|[] ]; rewrite <- H.
+    apply Z.arithmetic_shiftr1_bound.
+    pose proof nth_default_preserves_properties _ f (n - 1) 0 Hf H1;
+      simpl in H0; Z.solve_range. Qed.
+
+Lemma sat_arithmetic_shiftr1_length m n f
+      (Hn : (0 < n)%nat)
+      (Hf : length f = n) :
+  length (sat_arithmetic_shiftr1 m n f) = n.
+Proof. unfold sat_arithmetic_shiftr1; rewrite app_length, map_length, seq_length;
+         simpl; lia. Qed.
+
+Lemma sat_arithmetic_shiftr_iter_sat_arithmetic_shiftr1 machine_wordsize n f k
+      (Hn : (0 < n)%nat)
+      (Hf : length f = n)
+      (Hk : 0 <= k < machine_wordsize)
+      (Hf2 : forall z, In z f -> 0 <= z < 2^machine_wordsize) :
+  sat_arithmetic_shiftr machine_wordsize n f k
+  = iter_sat_arithmetic_shiftr1 machine_wordsize n f (Z.abs_nat k).
+Proof.
+  assert (0 < 2 ^ machine_wordsize) by (apply Z.pow_pos_nonneg; lia).
+  assert (Hm : 0 <= machine_wordsize) by lia.
+  destruct (Z.abs_nat k) as [|m] eqn:E.
+  - replace k with 0 by lia; simpl; apply sat_arithmetic_shiftr_0; try assumption; lia.
+  - generalize dependent k. generalize dependent f.
+    induction m; intros.
+    + simpl; replace k with (0 + 1) by lia.
+      rewrite sat_arithmetic_shiftr_1 by (try assumption; lia). reflexivity.
+    + specialize (IHm (sat_arithmetic_shiftr1 machine_wordsize n f)
+                      (sat_arithmetic_shiftr1_length machine_wordsize n f Hn Hf)
+                      (sat_arithmetic_shiftr_bound machine_wordsize n f Hm Hf2)
+                      (k - 1) ltac:(lia) ltac:(lia)).
+      rewrite iter_sat_arithmetic_shiftr_S, <- IHm.
+      rewrite sat_arithmetic_shiftr_sat_arithmetic_shiftr1
+        by (try lia; assumption).
+      rewrite Z.sub_simpl_r; reflexivity. Qed.
+
+Lemma eval_sat_arithmetic_shiftr machine_wordsize n f k
+      (Hn : (0 < n)%nat)
+      (Hf : length f = n)
+      (Hk : 0 <= k < machine_wordsize)
+      (Hf2 : forall z, In z f -> 0 <= z < 2^machine_wordsize) :
+  eval_twos_complement machine_wordsize n
+                       (sat_arithmetic_shiftr machine_wordsize n f k) =
+  eval_twos_complement machine_wordsize n f / (2 ^ k).
+Proof.
+  assert (Hm : 0 <= machine_wordsize) by lia.
+  rewrite sat_arithmetic_shiftr_iter_sat_arithmetic_shiftr1 by assumption.
+  destruct (Z.abs_nat k) as [|m] eqn:E.
+  - replace k with 0 by lia; simpl; rewrite Z.div_1_r; reflexivity.
+  - generalize dependent k; generalize dependent f; induction m; intros.
+    + simpl; replace k with 1 by lia; rewrite Z.pow_1_r.
+      apply eval_twos_complement_sat_arithmetic_shiftr1; try assumption; lia.
+    + rewrite iter_sat_arithmetic_shiftr_S.
+      specialize (IHm (sat_arithmetic_shiftr1 machine_wordsize n f)
+                      (sat_arithmetic_shiftr1_length machine_wordsize n f Hn Hf)
+                      (sat_arithmetic_shiftr_bound machine_wordsize n f Hm Hf2)
+                      (k - 1) ltac:(lia) ltac:(lia)).
+      assert (0 < 2 ^ (k - 1)) by (apply Z.pow_pos_nonneg; lia).
+      rewrite IHm, eval_twos_complement_sat_arithmetic_shiftr1 by (try assumption; lia).
+      rewrite Z.div_div, Z.pow_mul_base, Z.sub_simpl_r by lia; reflexivity. Qed.
+
+(** Section for firstn *)
+Lemma firstn_eval m n f k
+      (Hm : 0 < m)
+      (Hf : length f = n)
+      (Hf2 : forall z : Z, In z f -> 0 <= z < 2 ^ m)
+      (Hk : (k <= n)%nat) :
+  Positional.eval (uweight m) k (firstn k f) = Positional.eval (uweight m) n f mod 2 ^ (m * k).
+Proof.
+  rewrite <- (firstn_skipn k f) at 2.
+  replace n with (k + length (skipn k f))%nat by (rewrite skipn_length; lia).
+  rewrite (uweight_eval_app' m ltac:(lia) k), uweight_eq_alt, <- Z.pow_mul_r
+    by (rewrite ?firstn_length, ?Nat.min_l; lia).
+  autorewrite with push_Zmod.
+  rewrite Z.mod_0_l, Z.add_0_r,  Z.mod_mod
+    by (try apply Z.pow_nonzero; nia).
+  rewrite Z.mod_small. reflexivity.
+  apply eval_bound. lia. intros.
+  apply Hf2. apply (In_firstn k).  assumption.
+  rewrite firstn_length, Nat.min_l. reflexivity. lia. Qed.
+
+Local Notation eval m n f := (Positional.eval (uweight m) n f).
+
+(** sat_ones section *)
+Lemma sat_ones_spec m n
+      (Hm : 0 <= m) :
+  eval m n (sat_ones m n) = Z.ones (m * n).
+Proof.
+  unfold sat_ones. induction n.
+  - rewrite Z.mul_0_r; reflexivity.
+  - simpl.
+    rewrite eval_cons, uweight_eval_shift by (try apply repeat_length; lia).
+    rewrite IHn, uweight_0, uweight_eq_alt, Z.pow_1_r by lia.
+    rewrite !Z.ones_equiv, <- !Z.sub_1_r. ring_simplify.
+    rewrite <- Z.pow_add_r by lia. repeat apply f_equal2; lia. Qed.
+
+(** sat_sign_extend section *)
+Lemma sat_sign_extend_eval m n_old n_new f
+      (Hn_old : (0 < n_old)%nat)
+      (Hn_new : (n_old <= n_new)%nat)
+      (Hf : (length f = n_old))
+      (Hm : 0 < m)
+      (Hf2 : forall z : Z, In z f -> 0 <= z < 2 ^ m) :
+  Positional.eval (uweight m) n_new (sat_sign_extend m n_old n_new f)
+  = Z.sign_extend (m * n_old) (m * n_new) (Positional.eval (uweight m) n_old f).
+Proof.
+  rewrite Z.sign_extend_add by (solve [ nia | apply eval_bound; assumption ]).
+  unfold sat_sign_extend; rewrite unfold_Let_In, Zselect.Z.zselect_correct.
+  rewrite Z.sign_bit_testbit
+    by (solve [ lia | apply nth_default_preserves_properties; try assumption; Z.solve_range]).
+  rewrite eval_testbit by (solve [ assumption | nia ]). 
+  assert (H : (Z.abs_nat ((m * Z.of_nat n_old - 1) / m)) = (n_old - 1)%nat).
+  { unfold Z.sub. rewrite Z.div_add_l' by lia.
+    assert (H2 : ((- (1)) / m) = - (1)).
+    destruct (dec (m = 1)); subst; [reflexivity|].
+    rewrite Z_div_nz_opp_full, Z.div_small by (rewrite ?Z.mod_1_l; lia); lia. rewrite H2; lia. }
+  assert (H1 : (m * Z.of_nat n_old - 1) mod m = m - 1).
+  { destruct (dec (m = 1)); subst; [now rewrite Z.mod_1_r|].
+    repeat (pull_Zmod; push_Zmod). rewrite Z.mod_1_l, Z.mod_neg_small; lia. }
+  rewrite H, H1.
+  destruct (Z.testbit (nth_default 0 f (n_old - 1)) (m - 1)); simpl.
+  -  rewrite (uweight_eval_app) with (n := (n_old)%nat) by (rewrite ?repeat_length; lia).
+     rewrite repeat_length. fold (sat_ones m (n_new - n_old)).
+     rewrite sat_ones_spec,  uweight_eq_alt by lia. unfold Z.ones_at. rewrite Z.shiftl_mul_pow2 by nia.
+     rewrite Z.pow_mul_r by lia.
+     replace (m * Z.of_nat (n_new - n_old)) with (m * Z.of_nat n_new - m * Z.of_nat n_old) by nia; lia.
+  - rewrite (uweight_eval_app) with (n := (n_old)%nat) by (rewrite ?repeat_length; lia).
+    rewrite repeat_length; fold (zeros (n_new - n_old)); rewrite eval_zeros; lia. Qed.
+
+Lemma sat_sign_extend_length m n_old n_new f
+      (Hn_old : (0 < n_old)%nat)
+      (Hn_new : (n_old <= n_new)%nat)
+      (Hf : (length f = n_old)) :
+  length (sat_sign_extend m n_old n_new f) = n_new.
+Proof. unfold sat_sign_extend; rewrite unfold_Let_In, app_length, repeat_length. lia. Qed.
+
+Hint Rewrite sat_sign_extend_length : distr_length.
+
+(** sat_mul section *)
+Lemma sat_mul_bounds machine_wordsize n1 n2 f g
+      (mw0 : 0 < machine_wordsize)
+      (Hn2 : (0 < n2)%nat)
+      (Hf : length f = n1)
+      (Hg : length g = n1) :
+  forall z, In z (sat_mul machine_wordsize n1 n2 f g) -> 0 <= z < 2 ^ machine_wordsize.
+Proof.
+  intros z H; unfold sat_mul in *.
+  rewrite Rows.mul_partitions in * by (try apply uwprops; try apply Z.pow_nonzero; lia).
+  unfold Partition.partition in H. apply ListAux.in_map_inv in H.
+  destruct H as [a [H]]. rewrite H0, !uweight_eq_alt; try lia.
+  split.
+  - apply Z.div_le_lower_bound;
+      ring_simplify; try apply Z.mod_pos_bound;
+        apply Z.pow_pos_nonneg; try lia; apply Z.pow_pos_nonneg; lia.
+  - apply Z.div_lt_upper_bound.
+    apply Z.pow_pos_nonneg; try lia; apply Z.pow_pos_nonneg; lia.
+    replace ((_ ^ _) ^ _ * _) with ((2 ^ machine_wordsize) ^ Z.of_nat (S a)).
+    apply Z.mod_pos_bound; apply Z.pow_pos_nonneg; try lia; apply Z.pow_pos_nonneg; lia.
+    rewrite Z.mul_comm, Pow.Z.pow_mul_base;
+      try (replace (Z.of_nat (S a)) with ((Z.of_nat a + 1)) by lia; lia). Qed.
+
+Theorem sat_twos_complement_mul_correct m na nb nab a b
+        (Hm : 0 < m)
+        (Hna : (0 < na <= nab)%nat)
+        (Hnb : (0 < nb <= nab)%nat)
+        (Ha : length a = na)
+        (Hb : length b = nb)
+        (Ha2 : forall z : Z, In z a -> 0 <= z < 2 ^ m)
+        (Hb2 : forall z : Z, In z b -> 0 <= z < 2 ^ m)
+        (Hab_overflow : - 2 ^ (m * Z.of_nat nab - 1) <=
+                        Z.twos_complement (m * Z.of_nat na) (eval m na a) * Z.twos_complement (m * Z.of_nat nb) (eval m nb b) <
+                        2 ^ (m * Z.of_nat nab - 1)) :
+  eval_twos_complement m (nab) (sat_twos_complement_mul m na nb nab a b) =
+  (eval_twos_complement m na a) * (eval_twos_complement m nb b).
+Proof.
+  pose proof (uwprops m Hm).
+  pose proof (eval_bound m na a Hm Ha2 Ha).
+  pose proof (eval_bound m nb b Hm Hb2 Hb).
+  unfold sat_twos_complement_mul, eval_twos_complement.
+  rewrite (firstn_eval m (2 * nab)), Rows.mul_partitions, !sat_sign_extend_eval, eval_partition, Z.twos_complement_mod.
+  rewrite Z.mod_small.
+  fold (Z.twos_complement_mul_aux (m * na) (m * nb) (m * nab) (eval m na a) (eval m nb b)).
+  rewrite Z.twos_complement_mul_aux_spec by nia. reflexivity.
+  pose proof (Z.sign_extend_bound (m * na) (m * nab) (eval m na a) ltac:(nia) ltac:(nia) ltac:(assumption)).
+  pose proof (Z.sign_extend_bound (m * nb) (m * nab) (eval m nb b) ltac:(nia) ltac:(nia) ltac:(assumption)).
+  rewrite uweight_eq_alt.
+  replace ((2 ^ m) ^ Z.of_nat (2 * nab)) with (2 ^ (m * Z.of_nat nab) * 2 ^ (m * Z.of_nat nab)) by
+      (rewrite <- Z.pow_mul_r, <- Z.pow_add_r by nia; apply f_equal; nia). all: try nia; try assumption.
+  apply Z.pow_nonzero; lia. distr_length. distr_length.
+  apply Rows.length_mul; try assumption; distr_length.
+  apply sat_mul_bounds; distr_length; lia. Qed.
+
+Theorem sat_twos_complement_mul_full_correct m na nb a b
+        (Hm : 0 < m)
+        (Hna : (0 < na)%nat)
+        (Hnb : (0 < nb)%nat)
+        (Ha : length a = na)
+        (Hb : length b = nb)
+        (Ha2 : forall z : Z, In z a -> 0 <= z < 2 ^ m)
+        (Hb2 : forall z : Z, In z b -> 0 <= z < 2 ^ m) :
+  eval_twos_complement m (na + nb) (sat_twos_complement_mul_full m na nb a b) =
+  (eval_twos_complement m na a) * (eval_twos_complement m nb b).
+Proof.
+  unfold sat_twos_complement_mul_full. apply sat_twos_complement_mul_correct; try assumption; try lia.
+  pose proof (Z.twos_complement_bounds (m * Z.of_nat na) (eval m na a)).
+  pose proof (Z.twos_complement_bounds (m * Z.of_nat nb) (eval m nb b)).
+  assert (2 ^ (m * Z.of_nat na - 1) * 2 ^ (m * Z.of_nat nb - 1) < 2 ^ (m * Z.of_nat (na + nb) - 1)).
+  rewrite <- Z.pow_add_r by nia. apply Z.pow_lt_mono_r; nia. nia. Qed.
+
+Theorem word_sat_mul_correct m n a b
+        (Hm : 0 < m)
+        (Hn : (0 < n)%nat)
+        (Ha : 0 <= a < 2 ^ m)
+        (Hb : length b = n)
+        (Hb2 : forall z : Z, In z b -> 0 <= z < 2 ^ m) :
+  eval_twos_complement m (1 + n) (word_sat_mul m n a b) =
+  (Z.twos_complement m a) * eval_twos_complement m n b.
+Proof.
+  unfold word_sat_mul.
+  replace (Z.twos_complement m a) with (eval_twos_complement m 1 [a]).
+  apply sat_twos_complement_mul_full_correct; try assumption; try lia; try reflexivity.
+  intros z Hin; destruct Hin as [|[]]; subst; assumption.
+  unfold eval_twos_complement.
+  apply f_equal2; [lia|]; rewrite eval_cons, uweight_0, uweight_eval_shift, eval_nil, uweight_1; try reflexivity; lia. Qed.
+
+(** Correctness of wordsized divstep *)
+Theorem twos_complement_word_full_divstep_correct
+        machine_wordsize d f g u v q r
+        (fodd : Z.odd f = true)
+        (mw1 : 2 < machine_wordsize)
+        (overflow_d : - 2 ^ (machine_wordsize - 1) + 1 <
+                      Z.twos_complement machine_wordsize d <
+                      2 ^ (machine_wordsize - 1) - 1)
+        (overflow_f : - 2 ^ (machine_wordsize - 2) <
+                      Z.twos_complement machine_wordsize f <
+                      2 ^ (machine_wordsize - 2))
+        (overflow_g : - 2 ^ (machine_wordsize - 2) <
+                      Z.twos_complement machine_wordsize g <
+                      2 ^ (machine_wordsize - 2))
+        (overflow_u : - 2 ^ (machine_wordsize - 2) <
+                      Z.twos_complement machine_wordsize u <
+                      2 ^ (machine_wordsize - 2))
+        (overflow_v : - 2 ^ (machine_wordsize - 2) <
+                      Z.twos_complement machine_wordsize v <
+                      2 ^ (machine_wordsize - 2))
+        (overflow_q : - 2 ^ (machine_wordsize - 2) <
+                      Z.twos_complement machine_wordsize q <
+                      2 ^ (machine_wordsize - 2))
+        (overflow_r : - 2 ^ (machine_wordsize - 2) <
+                      Z.twos_complement machine_wordsize r <
+                      2 ^ (machine_wordsize - 2))
+        (Hf2 : 0 <= f < 2^machine_wordsize)
+        (Hg2 : 0 <= g < 2^machine_wordsize) :
+  let '(d1,f1,g1,u1,v1,q1,r1) :=
+      (twos_complement_word_full_divstep machine_wordsize d f g u v q r) in
+  (Z.twos_complement machine_wordsize d1,
+   Z.twos_complement machine_wordsize f1,
+   Z.twos_complement machine_wordsize g1,
+   Z.twos_complement machine_wordsize u1,
+   Z.twos_complement machine_wordsize v1,
+   Z.twos_complement machine_wordsize q1,
+   Z.twos_complement machine_wordsize r1) =
+  divstep_spec_full' (Z.twos_complement machine_wordsize d)
+                     (Z.twos_complement machine_wordsize f)
+                     (Z.twos_complement machine_wordsize g)
+                     (Z.twos_complement machine_wordsize u)
+                     (Z.twos_complement machine_wordsize v)
+                     (Z.twos_complement machine_wordsize q)
+                     (Z.twos_complement machine_wordsize r).
+Proof.
+  Arguments Z.add : simpl never.
+  assert (2 * 2 ^ (machine_wordsize - 2) = 2 ^ (machine_wordsize - 1)) by
+      (rewrite Z.pow_mul_base by lia; apply f_equal2; lia).
+  assert (2 ^ (machine_wordsize - 2) < 2^(machine_wordsize - 1)) by
+      (apply Z.pow_lt_mono_r; lia).
+  assert (2 <= 2 ^ (machine_wordsize - 2)) by
+      (replace 2 with (2 ^ 1) by lia; apply Z.pow_le_mono_r; lia).
+  unfold divstep_spec_full'; cbn -[Z.mul].
+  rewrite !Zselect.Z.zselect_correct.
+  rewrite !twos_complement_pos_spec, Zmod_odd, Z.twos_complement_odd by lia.
+  rewrite Z.twos_complement_mod2, (Zmod_odd g) by lia.
+  destruct (0 <? Z.twos_complement machine_wordsize d);
+    destruct (Z.odd g) eqn:godd;
+    rewrite (Zmod_odd); cbn -[Z.mul];
+      rewrite ?godd; cbn -[Z.mul].
+  rewrite <- (Z.twos_complement_odd machine_wordsize), !twos_complement_opp_spec by lia;
+    rewrite Z.odd_opp, Z.twos_complement_odd, fodd by lia; cbn -[Z.mul].
+  all: (repeat apply f_equal2;
+        repeat rewrite 1?Z.twos_complement_mod, 1?Z.twos_complement_add_full, 1?Z.twos_complement_one,
+        1?Z.arithmetic_shiftr1_spec, 1?twos_complement_opp_spec, 1?Z.twos_complement_zero;
+        rewrite ?Z.twos_complement_one, ?twos_complement_opp_spec;
+        try apply Z.mod_pos_bound; try apply f_equal2; lia). Qed.
+
+
+
+
+
+
+
+
+
